mldsa: update F* extraction

libcrux-ml-dsa/proofs/fstar/extraction/Libcrux_ml_dsa.Types.fst
@@ -9,17 +9,17 @@ let impl_2__len (v_SIZE: usize) (_: Prims.unit) = v_SIZE
 
 let impl_4__len (v_SIZE: usize) (_: Prims.unit) = v_SIZE
 
-let impl_4__as_raw (v_SIZE: usize) (self: t_MLDSASignature v_SIZE) = self.f_value
+let impl_4__as_ref (v_SIZE: usize) (self: t_MLDSASignature v_SIZE) = self.f_value
 
 let impl_4__new (v_SIZE: usize) (value: t_Array u8 v_SIZE) =
   { f_value = value } <: t_MLDSASignature v_SIZE
 
-let impl__as_raw (v_SIZE: usize) (self: t_MLDSASigningKey v_SIZE) = self.f_value
+let impl__as_ref (v_SIZE: usize) (self: t_MLDSASigningKey v_SIZE) = self.f_value
 
 let impl__new (v_SIZE: usize) (value: t_Array u8 v_SIZE) =
   { f_value = value } <: t_MLDSASigningKey v_SIZE
 
-let impl_2__as_raw (v_SIZE: usize) (self: t_MLDSAVerificationKey v_SIZE) = self.f_value
+let impl_2__as_ref (v_SIZE: usize) (self: t_MLDSAVerificationKey v_SIZE) = self.f_value
 
 let impl_2__new (v_SIZE: usize) (value: t_Array u8 v_SIZE) =
   { f_value = value } <: t_MLDSAVerificationKey v_SIZE
